mont spec

libcrux-ml-kem/proofs/fstar/spec/Spec.Utils.fst
@@ -1,9 +1,8 @@
 module Spec.Utils
 #set-options "--fuel 0 --ifuel 1 --z3rlimit 100"
-open Spec.SHA3
 open FStar.Mul
 open Core
-  
+
 (** Utils *)
 let map_slice #a #b
   (f:(x:a -> b))
@@ -54,6 +53,8 @@ type t_Result a b =
   | Err: b -> t_Result a b
 
 (** Hash Function *)
+open Spec.SHA3
+
 val v_G (input: t_Slice u8) : t_Array u8 (sz 64)
 let v_G input = map_slice Lib.RawIntTypes.u8_to_UInt8 (sha3_512 (Seq.length input) (map_slice Lib.IntTypes.secret input))
 
@@ -87,7 +88,6 @@ let update_at_range_lemma #n
     introduce forall (i:nat {i < len}). Seq.index s i == Seq.index s' i
     with (assert ( Seq.index (Seq.slice s  0 len) i == Seq.index s  i 
                  /\ Seq.index (Seq.slice s' 0 len) i == Seq.index s' i ))  
-
  
 /// Bounded integers
 
@@ -101,9 +101,10 @@ let is_i32b_array (l:nat) (x:t_Slice i32) = forall i. i < Seq.length x ==> is_i3
 
 let nat_div_ceil (x:nat) (y:pos) : nat = if (x % y = 0) then x/y else (x/y)+1
 
-let lemma_mul_i16b (b1 b2: nat) (n1 n2: i16) 
+val lemma_mul_i16b (b1 b2: nat) (n1 n2: i16) 
     : Lemma (requires (is_i16b b1 n1 /\ is_i16b b2 n2 /\ b1 * b2 < pow2 31))
-      (ensures (range (v n1 * v n2) i32_inttype /\ is_i32b (b1 * b2) ((cast n1 <: i32) *! (cast n2 <: i32)))) =
+      (ensures (range (v n1 * v n2) i32_inttype /\ is_i32b (b1 * b2) ((cast n1 <: i32) *! (cast n2 <: i32))))
+let lemma_mul_i16b (b1 b2: nat) (n1 n2: i16) =
   if v n1 = 0 || v n2 = 0
   then ()
   else 
@@ -115,9 +116,150 @@ let lemma_mul_i16b (b1 b2: nat) (n1 n2: i16)
     lemma_mult_le_right b2 (abs (v n1)) b1;
     lemma_abs_bound (v n1 * v n2) (b1 * b2)
 
-let lemma_add_i16b (b1 b2:nat) (n1 n2:i16) :
+val lemma_add_i16b (b1 b2:nat) (n1 n2:i16) :
   Lemma (requires (is_i16b b1 n1 /\ is_i16b b2 n2 /\ b1 + b2 < pow2 15))
         (ensures (range (v n1 + v n2) i16_inttype /\
                   is_i16b (b1 + b2) (n1 +! n2)))
-  = ()
+let lemma_add_i16b (b1 b2:nat) (n1 n2:i16) = ()
 
+let mont_mul_red_i16 (x:i16) (y:i16) : i16=
+  let vlow = x *. y in
+  let k = vlow *. (neg 3327s) in
+  let k_times_modulus = cast (((cast k <: i32) *. 3329l) >>! 16l) <: i16 in
+  let vhigh = cast (((cast x <: i32) *. (cast y <: i32)) >>! 16l) <: i16 in
+  vhigh -. k_times_modulus
+
+let mont_red_i32 (x:i32) : i16 =
+  let vlow = cast x <: i16 in
+  let k = vlow *. (neg 3327s) in
+  let k_times_modulus = cast (((cast k <: i32) *. 3329l) >>! 16l) <: i16 in
+  let vhigh = cast (x >>! 16l) <: i16 in
+  vhigh -. k_times_modulus
+
+#push-options "--z3rlimit 900 --split_queries always"
+val lemma_mont_red_i32 (x:i32): Lemma
+  (requires (Spec.Utils.is_i32b (3328 * pow2 16) x))
+  (ensures (
+          let result:i16 = mont_red_i32 x in
+          Spec.Utils.is_i16b (3328 + 1665) result /\
+          (Spec.Utils.is_i32b (3328 * 3328) x ==> Spec.Utils.is_i16b 3328 result) /\
+          v result % 3329 == (v x * 169) % 3329))
+let lemma_mont_red_i32 (x:i32) =
+  let vlow = cast x <: i16 in
+  assert (v vlow == v x @% pow2 16);
+  let k = vlow *. (neg 3327s) in
+  assert (v k == ((v x @% pow2 16) * (- 3327)) @% pow2 16);
+  let k_times_modulus = (cast k <: i32) *. 3329l in
+  assert (v k_times_modulus == (v k * 3329));
+  let c = cast (k_times_modulus >>! 16l) <: i16 in
+  assert (v c == (((v k * 3329) / pow2 16) @% pow2 16));
+  assert (v c == (((v k * 3329) / pow2 16)));
+  assert (is_i16b 1665 c);
+  let vhigh = cast (x >>! 16l) <: i16 in
+  assert (v vhigh == v x / pow2 16);
+  assert (is_i16b 3328 vhigh);
+  assert (Spec.Utils.is_i32b (3328 * 3328) x ==> Spec.Utils.is_i16b 169 vhigh);
+  let result = vhigh -. c in
+  assert (is_i16b (3328 + 1665) result);
+  assert (Spec.Utils.is_i32b (3328 * 3328) x ==> Spec.Utils.is_i16b 3328 result);
+  calc ( == ) {
+      v k_times_modulus % pow2 16;
+      ( == ) { assert (v k_times_modulus == v k * 3329) }
+      (v k * 3329) % pow2 16;
+      ( == ) { assert (v k = ((v x @% pow2 16) * (-3327)) @% pow2 16) }
+      ((((v x @% pow2 16) * (-3327)) @% pow2 16) * 3329) % pow2 16;
+      ( == ) { Math.Lemmas.lemma_mod_mul_distr_l ((v x @% pow2 16) * (-3327)) 3329 (pow2 16) }
+      ((((v x @% pow2 16) * (-3327)) * 3329) % pow2 16);
+      ( == ) { Math.Lemmas.lemma_mod_mul_distr_r (v x @% pow2 16) (-3327 * 3329) (pow2 16) }
+      ((v x @% pow2 16) % pow2 16);
+      ( == ) { Math.Lemmas.lemma_mod_sub (v x) (pow2 16) 1 }
+      (v x) % pow2 16;
+    };
+    Math.Lemmas.modulo_add (pow2 16) (- (v k_times_modulus)) (v x) (v k_times_modulus);
+    assert ((v x - v k_times_modulus) % pow2 16 == 0);
+    calc ( == ) {
+      v result % 3329;
+      ( == ) { assert (v result == v vhigh - v c) }
+      (v x / pow2 16 - v k_times_modulus / pow2 16) % 3329;
+      ( == ) { Math.Lemmas.lemma_div_exact (v x - v k_times_modulus) (pow2 16) }
+      ((v x - v k_times_modulus) / pow2 16) % 3329;
+      ( == ) { assert ((pow2 16 * 169) % 3329 == 1) }
+      (((v x - v k_times_modulus) / pow2 16) * ((pow2 16 * 169) % 3329)) % 3329;
+      ( == ) { Math.Lemmas.lemma_mod_mul_distr_r ((v x - v k_times_modulus) / pow2 16)
+        (pow2 16 * 169)
+        3329 }
+      (((v x - v k_times_modulus) / pow2 16) * pow2 16 * 169) % 3329;
+      ( == ) { Math.Lemmas.lemma_div_exact (v x - v k_times_modulus) (pow2 16) }
+      ((v x - v k_times_modulus) * 169) % 3329;
+      ( == ) { assert (v k_times_modulus == (v k @% pow2 16) * 3329) }
+      ((v x * 169) - ((v k @% pow2 16) * 3329 * 169)) % 3329;
+      ( == ) { Math.Lemmas.lemma_mod_sub (v x * 169) 3329 ((v k @% pow2 16) * 169) }
+      (v x * 169) % 3329;
+    }
+#pop-options
+
+#push-options "--z3rlimit 1200 --split_queries always --z3refresh"
+val lemma_mont_mul_red_i16 (x y:i16): Lemma
+  (requires (Spec.Utils.is_i16b 3328 y))
+  (ensures (
+          let result:i16 = mont_mul_red_i16 x y in
+          Spec.Utils.is_i16b (3328 + 1665) result /\
+          v result % 3329 == (v x * v y * 169) % 3329))
+let lemma_mont_mul_red_i16 (x y:i16) =
+  let vlow = x *. y in
+  assert (v vlow == (v x * v y) @% pow2 16);
+  let k = vlow *. (neg 3327s) in
+  assert (v k == (((v x * v y) @% pow2 16) * (- 3327)) @% pow2 16);
+  let k_times_modulus = (cast k <: i32) *. 3329l in
+  assert (v k_times_modulus == (v k * 3329));
+  let c = cast (k_times_modulus >>! 16l) <: i16 in
+  assert (v c == (((v k * 3329) / pow2 16) @% pow2 16));
+  assert (v c == (((v k * 3329) / pow2 16)));
+  assert (is_i16b 1665 c);
+  let vhigh = cast (((cast x <: i32) *. (cast y <: i32)) >>! 16l) <: i16 in
+  lemma_mul_i16b (pow2 15) (pow2 15) x y;
+  assert (is_i32b (pow2 30) ((cast x <: i32) *. (cast y <: i32)));
+  assert (v x * v y <= pow2 30 /\ v x * v y >= - pow2 30);
+  assert (v x * v y < pow2 31 /\ v x * v y > - pow2 31);
+  assert (v vhigh == (((v x * v y) @% pow2 32) / pow2 16) @% pow2 16);
+  assert (v vhigh == (v x * v y) / pow2 16);
+  assert (is_i16b 3328 vhigh);
+
+  let result = vhigh -. c in
+  assert (is_i16b (3328 + 1665) result);
+  assert (Spec.Utils.is_i32b (3328 * 3328) x ==> Spec.Utils.is_i16b 3328 result);
+  calc ( == ) {
+      v k_times_modulus % pow2 16;
+      ( == ) { assert (v k_times_modulus == v k * 3329) }
+      (v k * 3329) % pow2 16;
+      ( == ) { assert (v k = (((v x * v y) @% pow2 16) * (-3327)) @% pow2 16) }
+      (((((v x * v y)  @% pow2 16) * (-3327)) @% pow2 16) * 3329) % pow2 16;
+      ( == ) { Math.Lemmas.lemma_mod_mul_distr_l (((v x * v y) @% pow2 16) * (-3327)) 3329 (pow2 16) }
+      (((((v x * v y) @% pow2 16) * (-3327)) * 3329) % pow2 16);
+      ( == ) { Math.Lemmas.lemma_mod_mul_distr_r ((v x * v y) @% pow2 16) (-3327 * 3329) (pow2 16) }
+      (((v x * v y) @% pow2 16) % pow2 16);
+      ( == ) { Math.Lemmas.lemma_mod_sub ((v x * v y)) (pow2 16) 1 }
+      ((v x * v y)) % pow2 16;
+    };
+    Math.Lemmas.modulo_add (pow2 16) (- (v k_times_modulus)) ((v x * v y)) (v k_times_modulus);
+    assert (((v x * v y) - v k_times_modulus) % pow2 16 == 0);
+    calc ( == ) {
+      v result % 3329;
+      ( == ) { assert (v result == v vhigh - v c) }
+      ((v x * v y) / pow2 16 - v k_times_modulus / pow2 16) % 3329;
+      ( == ) { Math.Lemmas.lemma_div_exact ((v x * v y) - v k_times_modulus) (pow2 16) }
+      (((v x * v y) - v k_times_modulus) / pow2 16) % 3329;
+      ( == ) { assert ((pow2 16 * 169) % 3329 == 1) }
+      ((((v x * v y) - v k_times_modulus) / pow2 16) * ((pow2 16 * 169) % 3329)) % 3329;
+      ( == ) { Math.Lemmas.lemma_mod_mul_distr_r (((v x * v y) - v k_times_modulus) / pow2 16)
+        (pow2 16 * 169)
+        3329 }
+      ((((v x * v y) - v k_times_modulus) / pow2 16) * pow2 16 * 169) % 3329;
+      ( == ) { Math.Lemmas.lemma_div_exact ((v x * v y) - v k_times_modulus) (pow2 16) }
+      (((v x * v y) - v k_times_modulus) * 169) % 3329;
+      ( == ) { assert (v k_times_modulus == (v k @% pow2 16) * 3329) }
+      (((v x * v y) * 169) - ((v k @% pow2 16) * 3329 * 169)) % 3329;
+      ( == ) { Math.Lemmas.lemma_mod_sub ((v x * v y) * 169) 3329 ((v k @% pow2 16) * 169) }
+      ((v x * v y) * 169) % 3329;
+    }
+#pop-options
